{
 "cells": [
  {
   "cell_type": "markdown",
   "metadata": {},
   "source": [
    "# 1.\n",
    "## (a)\n",
    "From the notes provided on class website, we know that\n",
    "$\\bigtriangledown_x x^TAx=2Ax$ &nbsp; &nbsp; &nbsp; and &nbsp; &nbsp; &nbsp; $\\bigtriangledown_x b^Tx=b$\n",
    "\n",
    "$\\therefore\\bigtriangledown_xf(x)=\\bigtriangledown\\frac{1}{2}x^TAx+\\bigtriangledown_xb^Tx=Ax+b$\n",
    "\n",
    "## (b)\n",
    "$\\bigtriangledown_xf(x)=\n",
    "\\bigtriangledown_xg(h(x))=\n",
    "\\begin{bmatrix}\n",
    "\\frac{\\partial}{\\partial x_1}g(h(x)) \\\\\n",
    "\\vdots \\\\\n",
    "\\frac{\\partial}{\\partial x_n}g(h(x))\n",
    "\\end{bmatrix}$\n",
    "\n",
    "$=\\begin{bmatrix}\n",
    "g'(h(x))\\frac{\\partial h(x)}{\\partial x_1} \\\\\n",
    "\\vdots \\\\\n",
    "g'(h(x))\\frac{\\partial h(x)}{\\partial x_n}\n",
    "\\end{bmatrix}=g'(h(x))\\bigtriangledown_xh(x)$\n",
    "\n",
    "## (c)\n",
    "$\\bigtriangledown^2_xf(x)=\\bigtriangledown^2_x(\\frac{1}{2}x^TAx+b^Tx)=\\bigtriangledown^2_x\\frac{1}{2}x^TAx+\\bigtriangledown^2_xb^Tx$\n",
    "\n",
    "$\\because\\bigtriangledown^2_x b^Tx=\n",
    "\\begin{bmatrix}\n",
    "\\frac{\\partial^2}{\\partial x_1\\partial x_1}b^Tx\\cdots\\frac{\\partial^2}{\\partial x_1\\partial x_n}b^Tx \\\\\n",
    "\\vdots \\qquad\\qquad \\vdots \\\\\n",
    "\\frac{\\partial^2}{\\partial x_n\\partial x_1}b^Tx\\cdots\\frac{\\partial^2}{\\partial x_n\\partial x_n}b^Tx \n",
    "\\end{bmatrix}=0$\n",
    "\n",
    "$\\bigtriangledown^2_x(\\frac{1}{2}x^TAx+b^Tx)=\\bigtriangledown^2_x(\\frac{1}{2}x^TAx)=A$\n",
    "\n",
    "## (d)\n",
    "$\\bigtriangledown_xg(a^Tx)=\n",
    "\\begin{bmatrix}\n",
    "\\frac{\\partial}{\\partial x_1}g(a^Tx) \\\\\n",
    "\\vdots \\\\\n",
    "\\frac{\\partial}{\\partial x_n}g(a^Tx)\n",
    "\\end{bmatrix}=\n",
    "\\begin{bmatrix}\n",
    "g'(a^Tx)\\frac{\\partial a^Tx}{\\partial x_1} \\\\\n",
    "\\vdots \\\\\n",
    "g'(a^Tx)\\frac{\\partial a^Tx}{\\partial x_n} \n",
    "\\end{bmatrix}\n",
    "$\n",
    "\n",
    "$=g'(a^Tx)\\bigtriangledown_x a^Tx=g'(a^Tx)a$\n",
    "\n",
    "$\\bigtriangledown_x^2g(a^Tx)=\n",
    "\\begin{bmatrix}\n",
    "\\frac{\\partial^2}{\\partial x_1 \\partial x_1}g(a^Tx)\\quad\\cdots\\quad\\frac{\\partial^2}{\\partial x_1 \\partial x_n}g(a^Tx)\\\\\n",
    "\\vdots \\qquad\\qquad\\qquad\\qquad \\vdots\\\\\n",
    "\\frac{\\partial^2}{\\partial x_n \\partial x_1}g(a^Tx)\\quad\\cdots\\quad\\frac{\\partial^2}{\\partial x_n \\partial x_n}g(a^Tx)\n",
    "\\end{bmatrix}$\n",
    "\n",
    "$=g''(a^Tx)\\cdot\n",
    "\\begin{bmatrix}\n",
    "a_1\\cdot a_1\\quad\\cdots\\quad a_1\\cdot a_n\\\\\n",
    "\\vdots \\qquad\\qquad \\vdots\\\\\n",
    "a_n\\cdot a_1\\quad\\cdots\\quad a_n\\cdot a_n\n",
    "\\end{bmatrix}$\n",
    "\n",
    "$=g''(a^Tx)\\cdot aa^T$\n",
    "\n",
    "# 2.\n",
    "## (a)\n",
    "$\\forall x,\\quad x^TAx=\\sum^n_{i=1}\\sum^n_{j=1}A_{ij}x_ix_j$\n",
    "\n",
    "$\\because A_{ij}=z_iz_j$\n",
    "\n",
    "$\\sum^n_{i=1}\\sum^n_{j=1}A_{ij}x_ix_j=\\sum^n_{i=1}\\sum^n_{j=1}z_iz_jx_ix_j$\n",
    "\n",
    "$=\\sum^n_{i=1}(z_ix_i)^2\\geq0$\n",
    "\n",
    "$\\therefore$ A is positive semidefinite\n",
    "\n",
    "## (b)\n",
    "$A=\\begin{bmatrix}\n",
    "z_1z_1 \\quad\\cdots\\quad z_1z_n\\\\\n",
    "z_2z_1 \\quad\\cdots\\quad z_2z_n\\\\\n",
    "\\vdots\\\\\n",
    "z_nz_1 \\quad\\cdots\\quad z_nz_n\n",
    "\\end{bmatrix}$\n",
    "\n",
    "row operatins (row i multiply $z_1/z_i$)\n",
    "$\\rightarrow A=\\begin{bmatrix}\n",
    "z_1z_1 \\quad\\cdots\\quad  z_1z_n\\\\\n",
    "0 \\quad\\quad\\cdots\\quad\\quad 0\\\\\n",
    "\\vdots\\\\\n",
    "0 \\quad\\quad\\cdots\\quad\\quad 0\n",
    "\\end{bmatrix}$\n",
    "\n",
    "$\\therefore$ rank of A equal 1\n",
    "\n",
    "From the dimension theory, we know that $rank + nullity = n$\n",
    "\n",
    "$\\therefore$ dimenesion of null space is n - 1\n",
    "\n",
    "Also, null space consists of orthogonal vectors of $z^T$, so $Ax=zz^Tx$ will be 0\n",
    "\n",
    "## (c)\n",
    "$\\forall x, \\quad x^TBAB^Tx = (xB^T)A(B^Tx)$\n",
    "\n",
    "Let $\\quad v = B^Tx$\n",
    "\n",
    "$v^TAv\\geq0$, since A is positive semidefinite.\n",
    "\n",
    "$\\therefore BAB^T$ is positive semidefinite.\n",
    "\n",
    "# 3.\n",
    "## (a)\n",
    "Since Matrix $T$ is invertible, $A=T\\Lambda T^{-1} \\rightarrow AT=\\Lambda T$\n",
    "\n",
    "$\\begin{bmatrix}\n",
    "    At^{(1)} \\quad At^{(2)} \\cdots At^{(n)}\n",
    "\\end{bmatrix}=\\begin{bmatrix}\n",
    "\\lambda^{(1)}t^{(1)} \\quad \\lambda^{(2)}t^{(2)} \\cdots \\lambda^{(n)}t^{(n)}\n",
    "\\end{bmatrix}$\n",
    "\n",
    "$\\therefore \\forall i=1 \\cdots n$, \n",
    "$At^{(i)}=\\lambda t^{(i)}$\n",
    "\n",
    "## (b)\n",
    "\n",
    "Follow the logic in problem 3(a)\n",
    "\n",
    "$AU = U\\Lambda  \\rightarrow Au^{(i)} = \\lambda ^ {(i)} u ^{(i)}$\n",
    "\n",
    "## (c)\n",
    "Since U is orthogonal matrix, so $U^Tu^{(i)} = e ^{(i)}$\n",
    "\n",
    "and A is PSD, so $u^{(i)T}U\\Lambda U^T u^{(i)} \\geq 0$\n",
    "\n",
    "Therefore, $ \\forall i, e^{(i)T}\\Lambda e^{(i)} = \\lambda(A) \\geq 0$"
   ]
  }
 ],
 "metadata": {
  "kernelspec": {
   "display_name": "Python 3",
   "language": "python",
   "name": "python3"
  },
  "language_info": {
   "codemirror_mode": {
    "name": "ipython",
    "version": 3
   },
   "file_extension": ".py",
   "mimetype": "text/x-python",
   "name": "python",
   "nbconvert_exporter": "python",
   "pygments_lexer": "ipython3",
   "version": "3.7.2"
  }
 },
 "nbformat": 4,
 "nbformat_minor": 2
}
